stdlib/lampe/Stdlib/Cmp.lean
@@ -1,15 +1,39 @@
 import «std-1.0.0-beta.12».Extracted
 import Lampe
 
+import Mathlib.Order.Compare
+import Stdlib.Tuple
+
 namespace Lampe.Stdlib.Cmp
 
 open «std-1.0.0-beta.12»
+open Lampe.Stdlib
 
 namespace Eq
 
+set_option Lampe.pp.Expr true
+set_option Lampe.pp.STHoare true
+
+/-- A shorthand for a call to the `std::cmp::Eq::eq` method. -/
+@[reducible]
+def eq {p} 
+    (generics : HList Kind.denote «std-1.0.0-beta.12::cmp::Eq».«#genericKinds»)
+    (Self : Tp)
+    (associatedTypes : HList Kind.denote «std-1.0.0-beta.12::cmp::Eq».«#associatedTypesKinds»)
+    (fnGenerics : HList Kind.denote «std-1.0.0-beta.12::cmp::Eq».«#genericKinds»)
+  : HList (Tp.denote p)
+      («std-1.0.0-beta.12::cmp::Eq».eq.«#inputs» generics Self associatedTypes fnGenerics)
+  → Expr (Tp.denote p)
+      («std-1.0.0-beta.12::cmp::Eq».eq.«#output» generics Self associatedTypes fnGenerics) :=
+  «std-1.0.0-beta.12::cmp::Eq».eq generics Self associatedTypes fnGenerics
+
+/-- Asserts that the provided `tp` has an implementation of `std::cmp::Eq` in the environment. -/
+@[reducible]
+def hasEqImpl (env : Env) (tp : Tp) := «std-1.0.0-beta.12::cmp::Eq».hasImpl env h![] tp
+
 theorem field_eq_spec {p a b}
   : STHoare p env ⟦⟧
-    («std-1.0.0-beta.12::cmp::Eq».eq h![] .field h![] h![] h![a, b])
+    (eq h![] .field h![] h![] h![a, b])
     fun r: Bool => ⟦r ↔ a = b⟧ := by
   resolve_trait
   steps
@@ -17,7 +41,7 @@ theorem field_eq_spec {p a b}
 
 theorem u128_eq_spec {p a b}
   : STHoare p env ⟦⟧
-    («std-1.0.0-beta.12::cmp::Eq».eq h![] (.u 128) h![] h![] h![a, b])
+    (eq h![] (.u 128) h![] h![] h![a, b])
     (fun r : Bool => r ↔ a = b) := by
   resolve_trait
   steps
@@ -25,7 +49,7 @@ theorem u128_eq_spec {p a b}
 
 theorem u64_eq_spec {p a b}
   : STHoare p env ⟦⟧
-    («std-1.0.0-beta.12::cmp::Eq».eq h![] (.u 64) h![] h![] h![a, b])
+    (eq h![] (.u 64) h![] h![] h![a, b])
     (fun r : Bool => r ↔ a = b) := by
   resolve_trait
   steps
@@ -33,7 +57,7 @@ theorem u64_eq_spec {p a b}
 
 theorem u32_eq_spec {p a b}
   : STHoare p env ⟦⟧
-    («std-1.0.0-beta.12::cmp::Eq».eq h![] (.u 32) h![] h![] h![a, b])
+    (eq h![] (.u 32) h![] h![] h![a, b])
     (fun r : Bool => r ↔ a = b) := by
   resolve_trait
   steps
@@ -41,7 +65,7 @@ theorem u32_eq_spec {p a b}
 
 theorem u16_eq_spec {p a b}
   : STHoare p env ⟦⟧
-    («std-1.0.0-beta.12::cmp::Eq».eq h![] (.u 16) h![] h![] h![a, b])
+    (eq h![] (.u 16) h![] h![] h![a, b])
     (fun r : Bool => r ↔ a = b) := by
   resolve_trait
   steps
@@ -49,7 +73,7 @@ theorem u16_eq_spec {p a b}
 
 theorem u8_eq_spec {p a b}
   : STHoare p env ⟦⟧
-    («std-1.0.0-beta.12::cmp::Eq».eq h![] (.u 8) h![] h![] h![a, b])
+    (eq h![] (.u 8) h![] h![] h![a, b])
     fun r : Bool => ⟦r ↔ a = b⟧ := by
   resolve_trait
   steps
@@ -57,7 +81,7 @@ theorem u8_eq_spec {p a b}
 
 theorem u1_eq_spec {p a b}
   : STHoare p env ⟦⟧
-    («std-1.0.0-beta.12::cmp::Eq».eq h![] (.u 1) h![] h![] h![a, b])
+    (eq h![] (.u 1) h![] h![] h![a, b])
     fun r : Bool => ⟦r ↔ a = b⟧ := by
   resolve_trait
   steps
@@ -65,7 +89,7 @@ theorem u1_eq_spec {p a b}
 
 theorem i8_eq_spec {p a b}
   : STHoare p env ⟦⟧
-    («std-1.0.0-beta.12::cmp::Eq».eq h![] (.i 8) h![] h![] h![a, b])
+    (eq h![] (.i 8) h![] h![] h![a, b])
     fun r : Bool => ⟦r ↔ a = b⟧ := by
   resolve_trait
   steps
@@ -73,7 +97,7 @@ theorem i8_eq_spec {p a b}
 
 theorem i16_eq_spec {p a b}
   : STHoare p env ⟦⟧
-    («std-1.0.0-beta.12::cmp::Eq».eq h![] (.i 16) h![] h![] h![a, b])
+    (eq h![] (.i 16) h![] h![] h![a, b])
     fun r : Bool => ⟦r ↔ a = b⟧ := by
   resolve_trait
   steps
@@ -81,7 +105,7 @@ theorem i16_eq_spec {p a b}
 
 theorem i32_eq_spec {p a b}
   : STHoare p env ⟦⟧
-    («std-1.0.0-beta.12::cmp::Eq».eq h![] (.i 32) h![] h![] h![a, b])
+    (eq h![] (.i 32) h![] h![] h![a, b])
     fun r : Bool => ⟦r ↔ a = b⟧ := by
   resolve_trait
   steps
@@ -89,7 +113,7 @@ theorem i32_eq_spec {p a b}
 
 theorem i64_eq_spec {p a b}
   : STHoare p env ⟦⟧
-    («std-1.0.0-beta.12::cmp::Eq».eq h![] (.i 64) h![] h![] h![a, b])
+    (eq h![] (.i 64) h![] h![] h![a, b])
     fun r : Bool => ⟦r ↔ a = b⟧ := by
   resolve_trait
   steps
@@ -97,7 +121,7 @@ theorem i64_eq_spec {p a b}
 
 theorem unit_eq_spec {p a b}
   : STHoare p env ⟦⟧
-    («std-1.0.0-beta.12::cmp::Eq».eq h![] (.unit) h![] h![] h![a, b])
+    (eq h![] (.unit) h![] h![] h![a, b])
     fun r : Bool => ⟦r ↔ a = b⟧ := by
   resolve_trait
   steps
@@ -105,7 +129,7 @@ theorem unit_eq_spec {p a b}
 
 theorem bool_eq_spec {p a b}
   : STHoare p env ⟦⟧
-    («std-1.0.0-beta.12::cmp::Eq».eq h![] (.bool) h![] h![] h![a, b])
+    (eq h![] (.bool) h![] h![] h![a, b])
     fun r : Bool => ⟦r ↔ a = b⟧ := by
   resolve_trait
   steps
@@ -113,12 +137,10 @@ theorem bool_eq_spec {p a b}
   · exact ()
 
 theorem array_eq_pure_spec {p T N a b}
-    {t_eq : «std-1.0.0-beta.12::cmp::Eq».hasImpl env h![] T}
-    {t_eq_f : ∀a b, STHoare p env ⟦⟧
-      («std-1.0.0-beta.12::cmp::Eq».eq h![] T h![] h![] h![a, b])
-      (fun r : Bool => ⟦r ↔ a = b⟧)}
+    {t_eq : hasEqImpl env T}
+    {t_eq_f : ∀a b, STHoare p env ⟦⟧ (eq h![] T h![] h![] h![a, b]) (fun r : Bool => ⟦r ↔ a = b⟧)}
   : STHoare p env ⟦⟧
-    («std-1.0.0-beta.12::cmp::Eq».eq h![] (T.array N) h![] h![] h![a, b])
+    (eq h![] (T.array N) h![] h![] h![a, b])
     (fun r : Bool => ⟦r ↔ a = b⟧) := by
   resolve_trait
   steps
@@ -167,12 +189,10 @@ theorem array_eq_pure_spec {p T N a b}
   exact Iff.intro (fun eq => List.Vector.eq _ _ eq) (fun eq => congrArg _ eq)
 
 theorem slice_eq_pure_spec {p T a b}
-    (h_trait_res : «std-1.0.0-beta.12::cmp::Eq».hasImpl env h![] T)
-    (h_eq_child: ∀a b, STHoare p env ⟦⟧
-      («std-1.0.0-beta.12::cmp::Eq».eq h![] T h![] h![] h![a, b])
-      fun r : Bool => ⟦r ↔ a = b⟧)
+    (h_trait_res : hasEqImpl env T)
+    (h_eq_child: ∀a b, STHoare p env ⟦⟧ (eq h![] T h![] h![] h![a, b]) fun r : Bool => ⟦r ↔ a = b⟧)
   : STHoare p env ⟦⟧
-    («std-1.0.0-beta.12::cmp::Eq».eq h![] T.slice h![] h![] h![a, b])
+    (eq h![] T.slice h![] h![] h![a, b])
     fun r : Bool => ⟦r ↔ a = b⟧ := by
   resolve_trait
   steps
@@ -223,23 +243,19 @@ theorem slice_eq_pure_spec {p T a b}
 theorem string_eq_pure_spec {p N a b}
     {u8_eq : «std-1.0.0-beta.12::cmp::Eq».hasImpl env h![] (.u 8)}
   : STHoare p env ⟦⟧
-    («std-1.0.0-beta.12::cmp::Eq».eq h![] (.str N) h![] h![] h![a, b])
+    (eq h![] (.str N) h![] h![] h![a, b])
     (fun r : Bool => ⟦r ↔ a = b⟧) := by
   resolve_trait
   steps [array_eq_pure_spec (t_eq := u8_eq) (t_eq_f := fun _ _ => u8_eq_spec)]
   simp_all only [BitVec.natCast_eq_ofNat, List.Vector.mk_toList]
 
 theorem tuple2_eq_pure_spec {p A B self other}
-    {A_eq : «std-1.0.0-beta.12::cmp::Eq».hasImpl env h![] A}
-    {B_eq : «std-1.0.0-beta.12::cmp::Eq».hasImpl env h![] B}
-    {A_eq_f : ∀a b, STHoare p env ⟦⟧
-      («std-1.0.0-beta.12::cmp::Eq».eq h![] A h![] h![] h![a, b])
-      (fun r : Bool => ⟦r ↔ a = b⟧)}
-    {B_eq_f : ∀a b, STHoare p env ⟦⟧
-      («std-1.0.0-beta.12::cmp::Eq».eq h![] B h![] h![] h![a, b])
-      (fun r : Bool => ⟦r ↔ a = b⟧)}
+    {A_eq : hasEqImpl env A}
+    {B_eq : hasEqImpl env B}
+    {A_eq_f : ∀a b, STHoare p env ⟦⟧ (eq h![] A h![] h![] h![a, b]) (fun r : Bool => ⟦r ↔ a = b⟧)}
+    {B_eq_f : ∀a b, STHoare p env ⟦⟧ (eq h![] B h![] h![] h![a, b]) (fun r : Bool => ⟦r ↔ a = b⟧)}
   : STHoare p env ⟦⟧
-    («std-1.0.0-beta.12::cmp::Eq».eq h![] (Tp.tuple none [A, B]) h![] h![] h![self, other])
+    (eq h![] (Tp.tuple none [A, B]) h![] h![] h![self, other])
     (fun r : Bool => ⟦r ↔ self = other⟧) := by
   resolve_trait
   steps [A_eq_f, B_eq_f]
@@ -252,20 +268,14 @@ theorem tuple2_eq_pure_spec {p A B self other}
   simp_all
 
 theorem tuple3_eq_pure_spec {p A B C self other}
-    {A_eq : «std-1.0.0-beta.12::cmp::Eq».hasImpl env h![] A}
-    {B_eq : «std-1.0.0-beta.12::cmp::Eq».hasImpl env h![] B}
-    {C_eq : «std-1.0.0-beta.12::cmp::Eq».hasImpl env h![] C}
-    {A_eq_f : ∀a b, STHoare p env ⟦⟧
-      («std-1.0.0-beta.12::cmp::Eq».eq h![] A h![] h![] h![a, b])
-      (fun r : Bool => ⟦r ↔ a = b⟧)}
-    {B_eq_f : ∀a b, STHoare p env ⟦⟧
-      («std-1.0.0-beta.12::cmp::Eq».eq h![] B h![] h![] h![a, b])
-      (fun r : Bool => ⟦r ↔ a = b⟧)}
-    {C_eq_f : ∀a b, STHoare p env ⟦⟧
-      («std-1.0.0-beta.12::cmp::Eq».eq h![] C h![] h![] h![a, b])
-      (fun r : Bool => ⟦r ↔ a = b⟧)}
+    {A_eq : hasEqImpl env A}
+    {B_eq : hasEqImpl env B}
+    {C_eq : hasEqImpl env C}
+    {A_eq_f : ∀a b, STHoare p env ⟦⟧ (eq h![] A h![] h![] h![a, b]) (fun r : Bool => ⟦r ↔ a = b⟧)}
+    {B_eq_f : ∀a b, STHoare p env ⟦⟧ (eq h![] B h![] h![] h![a, b]) (fun r : Bool => ⟦r ↔ a = b⟧)}
+    {C_eq_f : ∀a b, STHoare p env ⟦⟧ (eq h![] C h![] h![] h![a, b]) (fun r : Bool => ⟦r ↔ a = b⟧)}
   : STHoare p env ⟦⟧
-    («std-1.0.0-beta.12::cmp::Eq».eq h![] (Tp.tuple none [A, B, C]) h![] h![] h![self, other])
+    (eq h![] (Tp.tuple none [A, B, C]) h![] h![] h![self, other])
     (fun r : Bool => ⟦r ↔ self = other⟧) := by
   resolve_trait
   steps [A_eq_f, B_eq_f, C_eq_f]
@@ -280,24 +290,16 @@ theorem tuple3_eq_pure_spec {p A B C self other}
 
 set_option maxHeartbeats 500000 in
 theorem tuple4_eq_pure_spec {p A B C D self other}
-    {A_eq : «std-1.0.0-beta.12::cmp::Eq».hasImpl env h![] A}
-    {B_eq : «std-1.0.0-beta.12::cmp::Eq».hasImpl env h![] B}
-    {C_eq : «std-1.0.0-beta.12::cmp::Eq».hasImpl env h![] C}
-    {D_eq : «std-1.0.0-beta.12::cmp::Eq».hasImpl env h![] D}
-    {A_eq_f : ∀a b, STHoare p env ⟦⟧
-      («std-1.0.0-beta.12::cmp::Eq».eq h![] A h![] h![] h![a, b])
-      (fun r : Bool => ⟦r ↔ a = b⟧)}
-    {B_eq_f : ∀a b, STHoare p env ⟦⟧
-      («std-1.0.0-beta.12::cmp::Eq».eq h![] B h![] h![] h![a, b])
-      (fun r : Bool => ⟦r ↔ a = b⟧)}
-    {C_eq_f : ∀a b, STHoare p env ⟦⟧
-      («std-1.0.0-beta.12::cmp::Eq».eq h![] C h![] h![] h![a, b])
-      (fun r : Bool => ⟦r ↔ a = b⟧)}
-    {D_eq_f : ∀a b, STHoare p env ⟦⟧
-      («std-1.0.0-beta.12::cmp::Eq».eq h![] D h![] h![] h![a, b])
-      (fun r : Bool => ⟦r ↔ a = b⟧)}
+    {A_eq : hasEqImpl env A}
+    {B_eq : hasEqImpl env B}
+    {C_eq : hasEqImpl env C}
+    {D_eq : hasEqImpl env D}
+    {A_eq_f : ∀a b, STHoare p env ⟦⟧ (eq h![] A h![] h![] h![a, b]) (fun r : Bool => ⟦r ↔ a = b⟧)}
+    {B_eq_f : ∀a b, STHoare p env ⟦⟧ (eq h![] B h![] h![] h![a, b]) (fun r : Bool => ⟦r ↔ a = b⟧)}
+    {C_eq_f : ∀a b, STHoare p env ⟦⟧ (eq h![] C h![] h![] h![a, b]) (fun r : Bool => ⟦r ↔ a = b⟧)}
+    {D_eq_f : ∀a b, STHoare p env ⟦⟧ (eq h![] D h![] h![] h![a, b]) (fun r : Bool => ⟦r ↔ a = b⟧)}
   : STHoare p env ⟦⟧
-    («std-1.0.0-beta.12::cmp::Eq».eq h![] (Tp.tuple none [A, B, C, D]) h![] h![] h![self, other])
+    (eq h![] (Tp.tuple none [A, B, C, D]) h![] h![] h![self, other])
     (fun r : Bool => ⟦r ↔ self = other⟧) := by
   resolve_trait
   steps [A_eq_f, B_eq_f, C_eq_f, D_eq_f]
@@ -312,28 +314,18 @@ theorem tuple4_eq_pure_spec {p A B C D self other}
 
 set_option maxHeartbeats 1000000 in
 theorem tuple5_eq_pure_spec {p A B C D E self other}
-    {A_eq : «std-1.0.0-beta.12::cmp::Eq».hasImpl env h![] A}
-    {B_eq : «std-1.0.0-beta.12::cmp::Eq».hasImpl env h![] B}
-    {C_eq : «std-1.0.0-beta.12::cmp::Eq».hasImpl env h![] C}
-    {D_eq : «std-1.0.0-beta.12::cmp::Eq».hasImpl env h![] D}
-    {E_eq : «std-1.0.0-beta.12::cmp::Eq».hasImpl env h![] E}
-    {A_eq_f : ∀a b, STHoare p env ⟦⟧
-      («std-1.0.0-beta.12::cmp::Eq».eq h![] A h![] h![] h![a, b])
-      (fun r : Bool => ⟦r ↔ a = b⟧)}
-    {B_eq_f : ∀a b, STHoare p env ⟦⟧
-      («std-1.0.0-beta.12::cmp::Eq».eq h![] B h![] h![] h![a, b])
-      (fun r : Bool => ⟦r ↔ a = b⟧)}
-    {C_eq_f : ∀a b, STHoare p env ⟦⟧
-      («std-1.0.0-beta.12::cmp::Eq».eq h![] C h![] h![] h![a, b])
-      (fun r : Bool => ⟦r ↔ a = b⟧)}
-    {D_eq_f : ∀a b, STHoare p env ⟦⟧
-      («std-1.0.0-beta.12::cmp::Eq».eq h![] D h![] h![] h![a, b])
-      (fun r : Bool => ⟦r ↔ a = b⟧)}
-    {E_eq_f : ∀a b, STHoare p env ⟦⟧
-      («std-1.0.0-beta.12::cmp::Eq».eq h![] E h![] h![] h![a, b])
-      (fun r : Bool => ⟦r ↔ a = b⟧)}
+    {A_eq : hasEqImpl env A}
+    {B_eq : hasEqImpl env B}
+    {C_eq : hasEqImpl env C}
+    {D_eq : hasEqImpl env D}
+    {E_eq : hasEqImpl env E}
+    {A_eq_f : ∀a b, STHoare p env ⟦⟧ (eq h![] A h![] h![] h![a, b]) (fun r : Bool => ⟦r ↔ a = b⟧)}
+    {B_eq_f : ∀a b, STHoare p env ⟦⟧ (eq h![] B h![] h![] h![a, b]) (fun r : Bool => ⟦r ↔ a = b⟧)}
+    {C_eq_f : ∀a b, STHoare p env ⟦⟧ (eq h![] C h![] h![] h![a, b]) (fun r : Bool => ⟦r ↔ a = b⟧)}
+    {D_eq_f : ∀a b, STHoare p env ⟦⟧ (eq h![] D h![] h![] h![a, b]) (fun r : Bool => ⟦r ↔ a = b⟧)}
+    {E_eq_f : ∀a b, STHoare p env ⟦⟧ (eq h![] E h![] h![] h![a, b]) (fun r : Bool => ⟦r ↔ a = b⟧)}
   : STHoare p env ⟦⟧
-    («std-1.0.0-beta.12::cmp::Eq».eq h![] (Tp.tuple none [A, B, C, D, E]) h![] h![] h![self, other])
+    (eq h![] (Tp.tuple none [A, B, C, D, E]) h![] h![] h![self, other])
     (fun r : Bool => ⟦r ↔ self = other⟧) := by
   resolve_trait
   steps [A_eq_f, B_eq_f, C_eq_f, D_eq_f, E_eq_f]
@@ -346,9 +338,9 @@ theorem tuple5_eq_pure_spec {p A B C D E self other}
   simp_all only [Bool.and_eq_true, Prod.mk.injEq, and_true]
   tauto
 
-theorem ordering_eq_pure_spec {p self other}
+theorem ordering_eq_spec {p self other}
   : STHoare p env ⟦⟧
-    («std-1.0.0-beta.12::cmp::Eq».eq h![] («std-1.0.0-beta.12::cmp::Ordering».tp h![]) h![] h![] h![self, other])
+    (eq h![] («std-1.0.0-beta.12::cmp::Ordering».tp h![]) h![] h![] h![self, other])
     (fun r : Bool => ⟦r ↔ self = other⟧) := by
   resolve_trait
   steps
@@ -361,14 +353,32 @@ end Eq
 
 namespace Ord
 
-/--
-Convert a Lean ordering into a Noir `std-1.0.0-beta.12::cmp::Ordering`.
+set_option Lampe.pp.Expr true
+set_option Lampe.pp.STHoare true
 
-We recommend providng the user with `std-1.0.0-beta.12::cmp::Ordering`s at the boundary of the theorem for any
+abbrev NoirOrdering := «std-1.0.0-beta.12::cmp::Ordering».tp h![]
+
+/-- A shorthand for a call to the `std::cmp::Ord::cmp` method. -/
+@[reducible]
+def cmp {p}
+    (generics : HList Kind.denote «std-1.0.0-beta.12::cmp::Ord».«#genericKinds»)
+    (Self : Tp)
+    (associatedTypes : HList Kind.denote «std-1.0.0-beta.12::cmp::Ord».«#associatedTypesKinds»)
+    (fnGenerics : HList Kind.denote «std-1.0.0-beta.12::cmp::Ord».cmp.«#genericKinds»)
+  : HList (Tp.denote p) 
+      («std-1.0.0-beta.12::cmp::Ord».cmp.«#inputs» generics Self associatedTypes fnGenerics)
+  → Expr (Tp.denote p) 
+      («std-1.0.0-beta.12::cmp::Ord».cmp.«#output» generics Self associatedTypes fnGenerics) :=
+  «std-1.0.0-beta.12::cmp::Ord».cmp generics Self associatedTypes fnGenerics
+
+/--
+Convert a Lean ordering into a Noir `std::cmp::Ordering`.
+
+We recommend providng the user with `std::cmp::Ordering`s at the boundary of the theorem for any
 ordering values 'created' by the theorem.
 -/
 @[reducible]
-def fromOrdering {p} : Ordering → («std-1.0.0-beta.12::cmp::Ordering».tp h![] |>.denote p)
+def fromOrdering {p} : Ordering → (NoirOrdering.denote p)
 | .lt => (0, ())
 | .eq => (1, ())
 | .gt => (2, ())
@@ -376,39 +386,646 @@ def fromOrdering {p} : Ordering → («std-1.0.0-beta.12::cmp::Ordering».tp h![
 /--
 Convert a Noir `std-1.0.0-beta.12::cmp::Ordering` into a Lean ordering.
 
-We recommend converting user-provided `std-1.0.0-beta.12::cmp::Ordering`s from the user, and converting them
-within the theorem.
+We recommend converting user-provided `std-1.0.0-beta.12::cmp::Ordering`s from the user, and
+converting them within the theorem.
 
 Note that in order to ensure that `toOrdering` is total,
 -/
-def toOrdering {p} : («std-1.0.0-beta.12::cmp::Ordering».tp h![] |>.denote p) → Ordering
+def toOrdering {p} : (NoirOrdering.denote p) → Ordering
 | (n, ()) => match (n.cast : ZMod 3) with
   | 0 => .lt
   | 1 => .eq
   | 2 => .gt
 
-theorem less_spec {p} : STHoare p env ⟦⟧
-  («std-1.0.0-beta.12::cmp::Ordering::less».call h![] h![])
-  (fun r => r = fromOrdering .lt) := by
+/-- Constructs the type of an embedded function that compares two instances of an arbitrary type. -/
+@[reducible]
+def ordFuncOf {p} (tp : Tp) := tp.denote p → tp.denote p → Ordering
+
+/-- Asserts that the provided `tp` has an implementation of `std::cmp::Ord` in the environment. -/
+@[reducible]
+def hasOrdImpl (env : Env) (tp : Tp) := «std-1.0.0-beta.12::cmp::Ord».hasImpl env h![] tp
+
+/--
+A shorthand of the pure semantics for calling an embedded function implementing the ordering
+comparison between two `tp`s.
+-/
+@[reducible]
+def pureOrdSemantics {p} {tp : Tp} (env : Env) (emb : ordFuncOf tp) (a b : Tp.denote p tp) :=
+  STHoare p env ⟦⟧ (cmp h![] tp h![] h![] h![a, b]) (fun r => r = fromOrdering (emb a b))
+
+theorem less_spec {p}
+  : STHoare p env ⟦⟧
+    («std-1.0.0-beta.12::cmp::Ordering::less».call h![] h![])
+    (fun r => r = fromOrdering .lt) := by
   enter_decl
   steps
   subst_vars
   simp
 
-theorem equal_spec {p} : STHoare p env ⟦⟧
-  («std-1.0.0-beta.12::cmp::Ordering::equal».call h![] h![])
-  (fun r => r = fromOrdering .eq) := by
+theorem equal_spec {p}
+  : STHoare p env ⟦⟧
+    («std-1.0.0-beta.12::cmp::Ordering::equal».call h![] h![])
+    (fun r => r = fromOrdering .eq) := by
   enter_decl
   steps
   subst_vars
   simp
 
-theorem greater_spec {p} : STHoare p env ⟦⟧
-  («std-1.0.0-beta.12::cmp::Ordering::greater».call h![] h![])
-  (fun r => r = fromOrdering .gt) := by
+theorem greater_spec {p}
+  : STHoare p env ⟦⟧
+    («std-1.0.0-beta.12::cmp::Ordering::greater».call h![] h![])
+    (fun r => r = fromOrdering .gt) := by
   enter_decl
   steps
   subst_vars
   simp
+
+theorem u128_ord_spec {p self other}
+  : STHoare p env ⟦⟧
+    (cmp h![] (.u 128) h![] h![] h![self, other])
+    (fun r => r = fromOrdering (compare self other)) := by
+  resolve_trait
+  steps
+  apply STHoare.ite_intro
+  · intro
+    steps [less_spec]
+    subst_vars; congr 1
+    simp_all [compare, compareOfLessAndEq]
+  · intro
+    steps
+    apply STHoare.ite_intro
+    · intro
+      steps [greater_spec]
+      subst_vars; congr 1
+      simp_all only [decide_eq_false_iff_not, BitVec.not_lt, gt_iff_lt, decide_eq_true_eq, compare,
+        compareOfLessAndEq]
+      rename_i leq lt
+
+      have h1 : ¬(self = other) := by
+        by_contra! h
+        subst h
+        simp_all only [BitVec.le_refl, BitVec.lt_irrefl]
+
+      have h2 : ¬(self < other) := by simp_all
+
+      simp_all
+    · intro
+      steps [equal_spec]
+      subst_vars; congr 1
+      simp_all [compare, compareOfLessAndEq]
+
+      have h1 : self = other := by
+        rename_i a b
+        apply BitVec.le_antisymm b a
+
+      have h2 : ¬(self < other) := by
+        simp_all
+
+      simp_all
+
+theorem u64_ord_spec {p self other}
+  : STHoare p env ⟦⟧
+    (cmp h![] (.u 64) h![] h![] h![self, other])
+    (fun r => r = fromOrdering (compare self other)) := by
+  resolve_trait
+  steps
+  apply STHoare.ite_intro
+  · intro
+    steps [less_spec]
+    subst_vars; congr 1
+    simp_all [compare, compareOfLessAndEq]
+  · intro
+    steps
+    apply STHoare.ite_intro
+    · intro
+      steps [greater_spec]
+      subst_vars; congr 1
+      simp_all only [decide_eq_false_iff_not, BitVec.not_lt, gt_iff_lt, decide_eq_true_eq, compare,
+        compareOfLessAndEq]
+      rename_i leq lt
+
+      have h1 : ¬(self = other) := by
+        by_contra! h
+        subst h
+        simp_all only [BitVec.le_refl, BitVec.lt_irrefl]
+
+      have h2 : ¬(self < other) := by simp_all
+
+      simp_all
+    · intro
+      steps [equal_spec]
+      subst_vars; congr 1
+      simp_all [compare, compareOfLessAndEq]
+
+      have h1 : self = other := by
+        rename_i a b
+        apply BitVec.le_antisymm b a
+
+      have h2 : ¬(self < other) := by
+        simp_all
+
+      simp_all
+
+theorem u32_ord_spec {p self other}
+  : STHoare p env ⟦⟧
+    (cmp h![] (.u 32) h![] h![] h![self, other])
+    (fun r => r = fromOrdering (compare self other)) := by
+  resolve_trait
+  steps
+  apply STHoare.ite_intro
+  · intro
+    steps [less_spec]
+    subst_vars; congr 1
+    simp_all [compare, compareOfLessAndEq]
+  · intro
+    steps
+    apply STHoare.ite_intro
+    · intro
+      steps [greater_spec]
+      subst_vars; congr 1
+      simp_all only [decide_eq_false_iff_not, BitVec.not_lt, gt_iff_lt, decide_eq_true_eq, compare,
+        compareOfLessAndEq]
+      rename_i leq lt
+
+      have h1 : ¬(self = other) := by
+        by_contra! h
+        subst h
+        simp_all only [BitVec.le_refl, BitVec.lt_irrefl]
+
+      have h2 : ¬(self < other) := by simp_all
+
+      simp_all
+    · intro
+      steps [equal_spec]
+      subst_vars; congr 1
+      simp_all [compare, compareOfLessAndEq]
+
+      have h1 : self = other := by
+        rename_i a b
+        apply BitVec.le_antisymm b a
+
+      have h2 : ¬(self < other) := by
+        simp_all
+
+      simp_all
+
+theorem u16_ord_spec {p self other}
+  : STHoare p env ⟦⟧
+    (cmp h![] (.u 16) h![] h![] h![self, other])
+    (fun r => r = fromOrdering (compare self other)) := by
+  resolve_trait
+  steps
+  apply STHoare.ite_intro
+  · intro
+    steps [less_spec]
+    subst_vars; congr 1
+    simp_all [compare, compareOfLessAndEq]
+  · intro
+    steps
+    apply STHoare.ite_intro
+    · intro
+      steps [greater_spec]
+      subst_vars; congr 1
+      simp_all only [decide_eq_false_iff_not, BitVec.not_lt, gt_iff_lt, decide_eq_true_eq, compare,
+        compareOfLessAndEq]
+      rename_i leq lt
+
+      have h1 : ¬(self = other) := by
+        by_contra! h
+        subst h
+        simp_all only [BitVec.le_refl, BitVec.lt_irrefl]
+
+      have h2 : ¬(self < other) := by simp_all
+
+      simp_all
+    · intro
+      steps [equal_spec]
+      subst_vars; congr 1
+      simp_all [compare, compareOfLessAndEq]
+
+      have h1 : self = other := by
+        rename_i a b
+        apply BitVec.le_antisymm b a
+
+      have h2 : ¬(self < other) := by
+        simp_all
+
+      simp_all
+
+theorem u8_ord_spec {p self other}
+  : STHoare p env ⟦⟧
+    (cmp h![] (.u 8) h![] h![] h![self, other])
+    (fun r => r = fromOrdering (compare self other)) := by
+  resolve_trait
+  steps
+  apply STHoare.ite_intro
+  · intro
+    steps [less_spec]
+    subst_vars; congr 1
+    simp_all [compare, compareOfLessAndEq]
+  · intro
+    steps
+    apply STHoare.ite_intro
+    · intro
+      steps [greater_spec]
+      subst_vars; congr 1
+      simp_all only [decide_eq_false_iff_not, BitVec.not_lt, gt_iff_lt, decide_eq_true_eq, compare,
+        compareOfLessAndEq]
+      rename_i leq lt
+
+      have h1 : ¬(self = other) := by
+        by_contra! h
+        subst h
+        simp_all only [BitVec.le_refl, BitVec.lt_irrefl]
+
+      have h2 : ¬(self < other) := by simp_all
+
+      simp_all
+    · intro
+      steps [equal_spec]
+      subst_vars; congr 1
+      simp_all [compare, compareOfLessAndEq]
+
+      have h1 : self = other := by
+        rename_i a b
+        apply BitVec.le_antisymm b a
+
+      have h2 : ¬(self < other) := by
+        simp_all
+
+      simp_all
+
+theorem i8_ord_spec {p self other}
+  : STHoare p env ⟦⟧
+    (cmp h![] (.i 8) h![] h![] h![self, other])
+    (fun r => r = fromOrdering (compare self other)) := by
+  resolve_trait
+  steps
+  apply STHoare.ite_intro
+  · intro
+    steps [less_spec]
+    subst_vars; congr 1
+    simp_all [compare, compareOfLessAndEq]
+  · intro
+    steps
+    apply STHoare.ite_intro
+    · intro
+      steps [greater_spec]
+      subst_vars; congr 1
+      simp_all only [decide_eq_false_iff_not, BitVec.not_lt, gt_iff_lt, decide_eq_true_eq, compare,
+        compareOfLessAndEq]
+      rename_i leq lt
+
+      have h1 : ¬(self = other) := by
+        by_contra! h
+        subst h
+        simp_all only [BitVec.le_refl, BitVec.lt_irrefl]
+
+      have h2 : ¬(self < other) := by simp_all
+
+      simp_all
+    · intro
+      steps [equal_spec]
+      subst_vars; congr 1
+      simp_all [compare, compareOfLessAndEq]
+
+      have h1 : self = other := by
+        rename_i a b
+        apply BitVec.le_antisymm b a
+
+      have h2 : ¬(self < other) := by
+        simp_all
+
+      simp_all
+
+theorem i16_ord_spec {p self other}
+  : STHoare p env ⟦⟧
+    (cmp h![] (.i 16) h![] h![] h![self, other])
+    (fun r => r = fromOrdering (compare self other)) := by
+  resolve_trait
+  steps
+  apply STHoare.ite_intro
+  · intro
+    steps [less_spec]
+    subst_vars; congr 1
+    simp_all [compare, compareOfLessAndEq]
+  · intro
+    steps
+    apply STHoare.ite_intro
+    · intro
+      steps [greater_spec]
+      subst_vars; congr 1
+      simp_all only [decide_eq_false_iff_not, BitVec.not_lt, gt_iff_lt, decide_eq_true_eq, compare,
+        compareOfLessAndEq]
+      rename_i leq lt
+
+      have h1 : ¬(self = other) := by
+        by_contra! h
+        subst h
+        simp_all only [BitVec.le_refl, BitVec.lt_irrefl]
+
+      have h2 : ¬(self < other) := by simp_all
+
+      simp_all
+    · intro
+      steps [equal_spec]
+      subst_vars; congr 1
+      simp_all [compare, compareOfLessAndEq]
+
+      have h1 : self = other := by
+        rename_i a b
+        apply BitVec.le_antisymm b a
+
+      have h2 : ¬(self < other) := by
+        simp_all
+
+      simp_all
+
+theorem i32_ord_spec {p self other}
+  : STHoare p env ⟦⟧
+    (cmp h![] (.i 32) h![] h![] h![self, other])
+    (fun r => r = fromOrdering (compare self other)) := by
+  resolve_trait
+  steps
+  apply STHoare.ite_intro
+  · intro
+    steps [less_spec]
+    subst_vars; congr 1
+    simp_all [compare, compareOfLessAndEq]
+  · intro
+    steps
+    apply STHoare.ite_intro
+    · intro
+      steps [greater_spec]
+      subst_vars; congr 1
+      simp_all only [decide_eq_false_iff_not, BitVec.not_lt, gt_iff_lt, decide_eq_true_eq, compare,
+        compareOfLessAndEq]
+      rename_i leq lt
+
+      have h1 : ¬(self = other) := by
+        by_contra! h
+        subst h
+        simp_all only [BitVec.le_refl, BitVec.lt_irrefl]
+
+      have h2 : ¬(self < other) := by simp_all
+
+      simp_all
+    · intro
+      steps [equal_spec]
+      subst_vars; congr 1
+      simp_all [compare, compareOfLessAndEq]
+
+      have h1 : self = other := by
+        rename_i a b
+        apply BitVec.le_antisymm b a
+
+      have h2 : ¬(self < other) := by
+        simp_all
+
+      simp_all
+
+theorem i64_ord_spec {p self other}
+  : STHoare p env ⟦⟧
+    (cmp h![] (.i 64) h![] h![] h![self, other])
+    (fun r => r = fromOrdering (compare self other)) := by
+  resolve_trait
+  steps
+  apply STHoare.ite_intro
+  · intro
+    steps [less_spec]
+    subst_vars; congr 1
+    simp_all [compare, compareOfLessAndEq]
+  · intro
+    steps
+    apply STHoare.ite_intro
+    · intro
+      steps [greater_spec]
+      subst_vars; congr 1
+      simp_all only [decide_eq_false_iff_not, BitVec.not_lt, gt_iff_lt, decide_eq_true_eq, compare,
+        compareOfLessAndEq]
+      rename_i leq lt
+
+      have h1 : ¬(self = other) := by
+        by_contra! h
+        subst h
+        simp_all only [BitVec.le_refl, BitVec.lt_irrefl]
+
+      have h2 : ¬(self < other) := by simp_all
+
+      simp_all
+    · intro
+      steps [equal_spec]
+      subst_vars; congr 1
+      simp_all [compare, compareOfLessAndEq]
+
+      have h1 : self = other := by
+        rename_i a b
+        apply BitVec.le_antisymm b a
+
+      have h2 : ¬(self < other) := by
+        simp_all
+
+      simp_all
+
+theorem unit_ord_spec {p self other}
+  : STHoare p env ⟦⟧
+    (cmp h![] .unit h![] h![] h![self, other])
+    (fun r => r = fromOrdering (.eq)) := by
+  resolve_trait
+  steps [equal_spec]
+  simp_all
+
+theorem bool_ord_spec {p self other}
+  : STHoare p env ⟦⟧
+    (cmp h![] .bool h![] h![] h![self, other])
+    (fun r => r = fromOrdering (compare self other)) := by
+  resolve_trait
+  steps
+  apply STHoare.ite_intro
+  · intro
+    apply STHoare.ite_intro
+    · intro
+      steps [equal_spec]
+      simp_all
+    · intro
+      steps [greater_spec]
+      subst_vars
+      congr
+  · intro
+    apply STHoare.ite_intro
+    · intro
+      steps [less_spec]
+      subst_vars
+      congr
+    · intro
+      steps [equal_spec]
+      subst_vars
+      congr
+
+-- TODO Array
+
+-- TODO Slice
+
+theorem tuple2_ord_pure_spec {p A B self other}
+    {A_ord : hasOrdImpl env A}
+    {B_ord : hasOrdImpl env B}
+    {A_ord_emb : ordFuncOf A}
+    {B_ord_emb : ordFuncOf B}
+    {A_ord_f : ∀a b, pureOrdSemantics env A_ord_emb a b}
+    {B_ord_f : ∀a b, pureOrdSemantics env B_ord_emb a b}
+  : STHoare p env ⟦⟧
+    (cmp h![] (Tp.tuple none [A, B]) h![] h![] h![self, other])
+    (fun r => r = fromOrdering (Tuple.compare h![A_ord_emb, B_ord_emb] self other)) := by
+  resolve_trait
+  cases self
+  cases other
+
+  steps [A_ord_f, equal_spec, Eq.ordering_eq_spec]
+  · exact ()
+
+  apply STHoare.ite_intro
+  · intro
+    steps
+    simp [Tuple.compare]
+
+    simp_all only [Bool.not_eq_eq_eq_not, Bool.not_true, ne_eq, ite_not, Bool.false_eq_true,
+      false_iff]
+    rename_i a1 _ b1 _ _ _ _ _ _
+    have h : A_ord_emb a1 b1 ≠ .eq := by intro a; simp_all only [not_true_eq_false]
+    simp_all
+
+  · intro
+    steps [B_ord_f]
+  
+    simp_all only [Bool.not_eq_eq_eq_not, Bool.not_false, ne_eq, ite_not, iff_true]
+    rename_i a1 a2 b1 b2 _ _ _ _
+
+    generalize r : A_ord_emb a1 b1 = res at *
+    rename_i cond
+    cases h : res
+    · subst h
+      simp [fromOrdering] at cond
+      injection cond with h1
+      norm_num at h1
+    · cases h : B_ord_emb a2.1 b2.1
+      all_goals (simp [Tuple.compare, fromOrdering]; simp_all)
+    · subst h
+      simp [fromOrdering] at cond
+      injection cond with h1
+      apply sub_eq_zero_of_eq at h1
+      norm_num at h1
+
+theorem tuple3_ord_pure_spec {p A B C self other}
+    {A_ord : hasOrdImpl env A}
+    {B_ord : hasOrdImpl env B}
+    {C_ord : hasOrdImpl env C}
+    {A_ord_emb : ordFuncOf A}
+    {B_ord_emb : ordFuncOf B}
+    {C_ord_emb : ordFuncOf C}
+    {A_ord_f : ∀a b, pureOrdSemantics env A_ord_emb a b}
+    {B_ord_f : ∀a b, pureOrdSemantics env B_ord_emb a b}
+    {C_ord_f : ∀a b, pureOrdSemantics env C_ord_emb a b}
+  : STHoare p env ⟦⟧
+    (cmp h![] (Tp.tuple none [A, B, C]) h![] h![] h![self, other])
+    (fun r => r = fromOrdering (Tuple.compare h![A_ord_emb, B_ord_emb, C_ord_emb] self other)) := by
+  resolve_trait
+  steps [A_ord_f, equal_spec, Eq.ordering_eq_spec]
+  step_as 
+    ([result ↦ ⟨NoirOrdering, fromOrdering $ A_ord_emb self.1 other.1⟩]) 
+    (fun _ => [
+      result ↦ ⟨NoirOrdering, fromOrdering $ Tuple.compare h![A_ord_emb, B_ord_emb] 
+        (Tuple.mk h![self.1, self.2.1]) 
+        (Tuple.mk h![other.1, other.2.1])⟩
+    ])
+  · apply STHoare.ite_intro
+    · intro
+      steps [B_ord_f]
+      simp_all only [true_iff, Lens.modify, Option.get_some, Tuple.mk, Tuple.compare]
+      congr
+      repeat rw [Tuple.tail_head_eq_snd]
+      rename_i equality cond
+      repeat rw [Tuple.head_eq_fst] at equality
+      
+      generalize h1 : A_ord_emb self.1 other.1 = a_res at *
+      cases a_res
+      · simp [fromOrdering] at equality
+        injection equality with fst
+        norm_num at fst
+      · cases B_ord_emb self.2.1 other.2.1 <;> simp_all
+      · simp [fromOrdering] at equality
+        injection equality with fst
+        apply sub_eq_zero_of_eq at fst
+        norm_num at fst
+
+    · intro
+      steps
+      simp_all only [Bool.false_eq_true, false_iff, Tuple.mk]
+      rename_i equality cond
+      repeat rw [Tuple.head_eq_fst] at equality
+      congr
+      unfold Tuple.compare 
+      simp only
+
+      generalize A_ord_emb self.1 other.1 = a_res at *
+      cases a_res <;> simp_all
+  
+  steps [Eq.ordering_eq_spec, equal_spec]
+
+  step_as 
+    ([result ↦ ⟨NoirOrdering, fromOrdering $ Tuple.compare h![A_ord_emb, B_ord_emb] 
+        (Tuple.mk h![self.1, self.2.1]) 
+        (Tuple.mk h![other.1, other.2.1])⟩]) 
+    (fun _ => [ result ↦ ⟨NoirOrdering, 
+      fromOrdering $ Tuple.compare h![A_ord_emb, B_ord_emb, C_ord_emb] self other⟩])
+  · apply STHoare.ite_intro
+    · intro
+      steps [C_ord_f]
+      simp_all only [true_iff, Lens.modify, Option.get_some, Tuple.mk, Tuple.compare]
+      congr
+      repeat rw [Tuple.tail_tail_head_eq_third] at *
+      simp_all only [Tuple.mk, Lens.modify]
+      rename_i equality cond
+      
+      generalize A_ord_emb self.1 other.1 = a_res at *
+      generalize B_ord_emb self.2.1 other.2.1 = b_res at *
+      cases a_res
+      · simp [fromOrdering] at equality
+        injection equality with fst
+        norm_num at fst
+      · simp_all
+        cases b_res
+        · simp [fromOrdering] at equality
+          injection equality with fst
+          norm_num at fst
+        · cases C_ord_emb self.2.2.1 other.2.2.1 <;> simp_all
+        · simp [fromOrdering] at equality
+          injection equality with fst
+          apply sub_eq_zero_of_eq at fst
+          norm_num at fst
+      · simp [fromOrdering] at equality
+        injection equality with fst
+        apply sub_eq_zero_of_eq at fst
+        norm_num at fst
+
+    · intro
+      steps
+      simp_all only [Bool.false_eq_true, false_iff, Tuple.mk]
+      rename_i equality cond
+      repeat rw [Tuple.head_eq_fst] at *
+      congr 2
+
+      simp_all only [Tuple.compare]
+
+      generalize A_ord_emb self.1 other.1 = a_res at *
+      generalize B_ord_emb self.2.1 other.2.1 = b_res at *
+
+      cases a_res
+      · simp_all
+      · cases b_res <;> simp_all
+      · simp_all
+
+  steps
+  subst_vars
+  rfl
 
 end Ord
